# Atividade 5

- Victor Azadinho Miranda
- RA: 171042191

## Exercício 1

1. $f(x, y) = 2x^4y^3 - xy^2 + 3y + 1$
\begin{align*}
  \frac{df(x, y)}{dx} = &8x^3y^3 - y^2\\
  \frac{df(x, y)}{dy} = &6x^4y^2 - 2xy + 3
\end{align*}

2. $f(x, y) = (x^3 - y^2)^5$
\begin{align*}
  \Rightarrow f(x, y) = &\sum_{i = 0}^5\binom{5}{i}(x^3)^{5 - i}(y^2)^i\\
  \Rightarrow f(x, y) =
    &\frac{5!}{0!(5 - 0)!}(x^3)^5(-y^2)^0+\\
    &\frac{5!}{1!(5 - 1)!}(x^3)^4(-y^2)^1+\\
    &\frac{5!}{2!(5 - 2)!}(x^3)^3(-y^2)^2+\\
    &\frac{5!}{3!(5 - 3)!}(x^3)^2(-y^2)^3+\\
    &\frac{5!}{4!(5 - 4)!}(x^3)^1(-y^2)^4+\\
    &\frac{5!}{5!(5 - 5)!}(x^3)^0(-y^2)^5\\
  \Rightarrow f(x, y) = &x^{15} - 5x^{12}y^2 + 10x^9y^4 - 10x^6y^6 + 5x^3y^8 - y^{10}\\
  \frac{df(x, y)}{dx} = &15x^{14} - 60x^{11}y^2 + 90x^8y^4 - 60x^5y^6 + 15x^2y^8\\
  \frac{df(x, y)}{dy} = &10x^{12}y - 40x^9y^3 + 60x^6y^5 - 40x^3y^7 + 10y^9
\end{align*}

## Exercício 3

$f(x, y) = ln \sqrt{x^2 + y^2}$

\begin{align*}
  \frac{df(u)}{dx} = &\frac{df}{du} \cdot \frac{du}{dx}\\
  f = &ln(u)\\
  u = &\sqrt{x^2 + y^2}\\
  \frac{df}{du} = &\frac{1}{u}\\
  \frac{dg(v)}{dx} = &\frac{dg}{dv} \cdot \frac{dv}{dx}\\
  g = &\sqrt{v}\\
  v = &x^2 + y^2\\
  \frac{dg}{dv} = &\frac{1}{2\sqrt{v}}\\
  \frac{dv}{dx} = &2x\\
  \frac{dg(v)}{dx} = &\frac{1}{2\sqrt{v}} \cdot 2x\\
  \frac{du}{dx} = &\frac{x}{\sqrt{x^2 + y^2}}\\
  \frac{df(u)}{dx} = &\frac{1}{u} \cdot \frac{x}{\sqrt{x^2 + y^2}}\\
  \frac{df(x, y)}{dx} = &\frac{x}{x^2 + y^2}\\
  \frac{d^2f(x, y)}{dx^2} = &\frac{df(x, y)}{dx} (\frac{x}{x^2 + y^2})\\
  \frac{d\frac{f}{g}}{dx} = &\frac{\frac{df}{dx} \cdot g - \frac{dg}{dx} \cdot f}{g^2}\\
  f = &x\\
  \frac{df}{dx} = &1\\
  g = &x^2 + y^2\\
  \frac{dg}{dx} = &2x\\
  \frac{d\frac{f}{g}}{dx} = &\frac{1(x^2 + y^2) - 2xx}{(x^2 + y^2)^2}\\
  \frac{d^2f(x, y)}{dx^2} = &\frac{-x^2 + y^2}{(x^2 + y^2)^2}
\end{align*}

\begin{align*}
  \frac{df(u)}{dy} = &\frac{df}{du} \cdot \frac{du}{dy}\\
  f = &ln(u)\\
  u = &\sqrt{x^2 + y^2}\\
  \frac{df}{du} = &\frac{1}{u}\\
  \frac{dg(v)}{dy} = &\frac{dg}{dv} \cdot \frac{dv}{dy}\\
  g = &\sqrt{v}\\
  v = &x^2 + y^2\\
  \frac{dg}{dv} = &\frac{1}{2\sqrt{v}}\\
  \frac{dv}{dy} = &2y\\
  \frac{dg(v)}{dx} = &\frac{1}{2\sqrt{v}} \cdot 2y\\
  \frac{du}{dy} = &\frac{y}{\sqrt{x^2 + y^2}}\\
  \frac{df(u)}{dy} = &\frac{1}{u} \cdot \frac{y}{\sqrt{x^2 + y^2}}\\
  \frac{df(x, y)}{dy} = &\frac{y}{x^2 + y^2}\\
  \frac{d^2f(x, y)}{dy^2} = &\frac{df(x, y)}{dy} (\frac{y}{x^2 + y^2})\\
  \frac{d\frac{f}{g}}{dy} = &\frac{\frac{df}{dy} \cdot g - \frac{dg}{dy} \cdot f}{g^2}\\
  f = &y\\
  \frac{df}{dy} = &1\\
  g = &x^2 + y^2\\
  \frac{dg}{dy} = &2y\\
  \frac{d\frac{f}{g}}{dy} = &\frac{1(x^2 + y^2) - 2yy}{(x^2 + y^2)^2}\\
  \frac{d^2f(x, y)}{dy^2} = &\frac{x^2 - y^2}{(x^2 + y^2)^2}
\end{align*}

\begin{align*}
  \frac{d^2f(x, y)}{dx^2} + \frac{d^2f(x, y)}{dy^2} = &0\\
  \frac{-x^2 + y^2}{(x^2 + y^2)^2} + \frac{x^2 - y^2}{(x^2 + y^2)^2} = &0
\end{align*}