# Atividade 7

- Victor Azadinho Miranda
- RA: 171042191

## Exercício 1

1. $f(x, y) = \sqrt{x^2 + y^2},\ p(-4, 3)$
\begin{align*}
  \frac{df(x, y)}{dx} = &\frac{df(u)}{du} \cdot \frac{du}{dx}\\
  u = x^2 + y^2,\ f(u) = &\sqrt{u}\\
  \frac{df(u)}{du} = &(\sqrt{u})'\\
  = &(u^{\frac{1}{2}})'\\
  = &\frac{u^{-\frac{1}{2}}}{2}\\
  = &\frac{1}{2u^{\frac{1}{2}}}\\
  \Rightarrow \frac{df(u)}{du} = &\frac{1}{2\sqrt{u}}\\
  \frac{du}{dx} = &(x^2 + y^2)'\\
  \Rightarrow \frac{du}{dx} = &2x\\
  \frac{df(x, y)}{dx} = &\frac{1}{2\sqrt{u}} \cdot 2x\\
  = &\frac{1}{2\sqrt{x^2 + y^2}} \cdot 2x\\
  \Rightarrow \frac{df(x, y)}{dx} = &\frac{x}{\sqrt{x^2 + y^2}}\\
\end{align*}

\begin{align*}
  \frac{df(x, y)}{dy} = &\frac{df(u)}{du} \cdot \frac{du}{dy}\\
  u = x^2 + y^2,\ f(u) = &\sqrt{u}\\
  \frac{df(u)}{du} = &(\sqrt{u})'\\
  = &(u^{\frac{1}{2}})'\\
  = &\frac{u^{-\frac{1}{2}}}{2}\\
  = &\frac{1}{2u^{\frac{1}{2}}}\\
  \Rightarrow \frac{df(u)}{du} = &\frac{1}{2\sqrt{u}}\\
  \frac{du}{dy} = &(x^2 + y^2)'\\
  \Rightarrow \frac{du}{dy} = &2y\\
  \frac{df(x, y)}{dy} = &\frac{1}{2\sqrt{u}} \cdot 2y\\
  = &\frac{1}{2\sqrt{x^2 + y^2}} \cdot 2y\\
  \Rightarrow \frac{df(x, y)}{dy} = &\frac{y}{\sqrt{x^2 + y^2}}\\
\end{align*}

\begin{align*}
  \frac{df(-4, 3)}{dx} = &\frac{(-4)}{\sqrt{(-4)^2 + (3)^2}}\\
  = &\frac{-4}{\sqrt{16 + 9}}\\
  = &-\frac{4}{\sqrt{25}}\\
  = &-\frac{4}{5}\\
  \Rightarrow \frac{df(-4, 3)}{dx} = &-\frac{4}{5}
\end{align*}

\begin{align*}
  \frac{df(-4, 3)}{dy} = &\frac{(3)}{\sqrt{(-4)^2 + (3)^2}}\\
  = &\frac{3}{\sqrt{16 + 9}}\\
  = &\frac{3}{\sqrt{25}}\\
  = &\frac{3}{5}\\
  \Rightarrow \frac{df(-4, 3)}{dy} = &\frac{3}{5}
\end{align*}

\begin{align*}
  \nabla f(x, y) = &-\frac{4}{5}\vec{i} + \frac{3}{5}\vec{j}
\end{align*}

## Exercício 2

2. $f(x, y, z) = xy^2z^2,\ p(2, -1, 4),\ \vec{u} = \vec{i} + 2\vec{j} - 3\vec{k}$

\begin{align*}
  \| \vec{u} \| = &\sqrt{(1)^2 + (2)^2 + (-3)^2}\\
  = &\sqrt{1 + 4 + 9}\\
  = &\sqrt{14}\\
  \vec{v} = &\frac{\vec{u}}{\|\vec{u}\|}\\
  \Rightarrow \vec{v} = &\frac{1}{\sqrt{14}}\vec{i} + \frac{2}{\sqrt{14}}\vec{j} - \frac{3}{\sqrt{14}}\vec{k}
\end{align*}

\begin{align*}
  \frac{df(x, y, z)}{dx} = &y^2z^2\\
  \frac{df(2, -1, 4)}{dx} = &(-1)^2(4)^2\\
  = &1 \cdot 16\\
  \Rightarrow \frac{df(2, -1, 4)}{dx} = &16\\
  \frac{df(x, y, z)}{dy} = &2xyz^2\\
  \frac{df(2, -1, 4)}{dy} = &2(2)(-1)(4)^2\\
  = &4 \cdot -1 \cdot 16\\
  \Rightarrow \frac{df(2, -1, 4)}{dy} = &-64\\
  \frac{df(x, y, z)}{dz} = &2xy^2z\\
  \frac{df(2, -1, 4)}{dz} = &2(2)(-1)^2(4)\\
  = &4 \cdot 1 \cdot 4\\
  \Rightarrow \frac{df(2, -1, 4)}{dz} = &16
\end{align*}

\begin{align*}
  D_{\vec{v}}f(x, y, z) = \frac{df(x, y, z)}{dx} \cdot v_1 + \frac{df(x, y, z)}{dy} \cdot v_2 + \frac{df(x, y, z)}{dz} \cdot v_3\\
  D_{\vec{v}}f(2, -1, 4) = \frac{df(2, -1, 4)}{dx} \cdot v_1 + \frac{df(2, -1, 4)}{dy} \cdot v_2 + \frac{df(2, -1, 4)}{dz} \cdot v_3\\
  = &16 \cdot \frac{1}{\sqrt{14}} - 64 \cdot \frac{2}{\sqrt{14}} - 16 \cdot \frac{3}{\sqrt{14}}\\
  = &\frac{16}{\sqrt{14}} - \frac{128}{\sqrt{14}} - \frac{48}{\sqrt{14}}\\
  \Rightarrow D_{\vec{v}}f(2, -1, 4) = &\frac{160}{\sqrt{14}}
\end{align*}